

$$\begin{aligned}
AV_{m-1} &= V_m H_{m,m-1} = [v_1, \dots, v_m] \begin{bmatrix} h_{1,1} & h_{1,2} & \dots & h_{1,m-2} & h_{1,m-1} \\ h_{2,1} & h_{2,2} & & h_{2,m-2} & h_{2,m-1} \\ 0 & h_{3,2} & & h_{3,m-2} & h_{3,m-1} \\ \vdots & & \ddots & \vdots & \vdots \\ 0 & & \dots & h_{m-1,m-2} & h_{m-1,m-1} \\ & & & 0 & h_{m,m-1} \end{bmatrix} \\
&= \left[ \sum_{i=1}^2 h_{i,1} v_i, \quad \sum_{i=1}^3 h_{i,2} v_i, \quad \dots, \sum_{i=1}^{m-1} h_{i,m-2} v_i, \quad \sum_{i=1}^m h_{i,m-1} v_i \right] \\
&= \left[ \sum_{i=1}^2 h_{i,1} v_i, \quad \sum_{i=1}^3 h_{i,2} v_i, \quad \dots, \sum_{i=1}^{m-1} h_{i,m-2} v_i, \quad \sum_{i=1}^{m-1} h_{i,m-1} v_i \right] + h_{m,m-1} v_m e_{m-1}^T \\
&= V_{m-1} H_{m-1,m-1} + h_{m,m-1} v_m e_{m-1}^T
\end{aligned}$$

$$\begin{aligned}
V_{m-1}^T AV_{m-1} &= V_{m-1}^T V_{m-1} H_{m-1,m-1} + h_{m,m-1} V_{m-1}^T v_m e_{m-1}^T \\
V_{m-1}^T AV_{m-1} &= I H_{m-1,m-1} + 0 = H_{m-1,m-1}
\end{aligned}$$

$$AV_{m-1} = V_{m-1} H_{m-1,m-1}$$